F_mu_ref/logrel.v
@@ -14,11 +14,6 @@ Section logrel.
   Context {Σ : gFunctors}.
   Notation "# v" := (of_val v) (at level 20).
 
-  Class Val_to_IProp_Persistent (f : valC -n> iPropG lang Σ) :=
-    val_to_iprop_persistent : ∀ v : val, PersistentP (f v).
-
-  Arguments Val_to_IProp_Persistent /.
-
   (** Just to get nicer closed forms, we define extend_context_interp in three steps. *)
   Program Definition extend_context_interp_fun1
     (τi : valC -n> iPropG lang Σ)
@@ -156,13 +151,11 @@ Section logrel.
         {|
           cofe_mor_car :=
             λ w,
-            (∀ (τ'i : {f : (valC -n> iPropG lang Σ) |
-                       Val_to_IProp_Persistent f}),
+            (∀ (τ'i : {f : (valC -n> iPropG lang Σ) | ∀ v, PersistentP (f v)}%type),
                 □ (WP TApp (# w) @ ⊤ {{λ v, (τi (`τ'i) v)}}))%I
         |}
     |}.
   Next Obligation.
-  Proof.
     intros τ τ' x y Hxy; cbn; rewrite Hxy; trivial.
   Qed.
   Next Obligation.
@@ -187,16 +180,13 @@ Section logrel.
         |}
     |}.
   Next Obligation.
-  Proof.
     intros τi rec_appr n x y Hxy; rewrite Hxy; trivial.
   Qed.
   Next Obligation.
-  Proof.
     intros τi n f g Hfg x. cbn.
     apply always_ne, exist_ne =>w; rewrite Hfg; trivial.
   Qed.
   Next Obligation.
-  Proof.
     intros n τi τi' Hτi f x. cbn.
     apply always_ne, exist_ne =>w; rewrite Hτi; trivial.
   Qed.
@@ -220,7 +210,7 @@ Section logrel.
         cofe_mor_car := λ τi, fixpoint (interp_rec_pre τi)
       |}.
   Next Obligation.
-  Proof. intros n f g H; apply fixpoint_ne => z; rewrite H; trivial. Qed.
+    intros n f g H; apply fixpoint_ne => z; rewrite H; trivial. Qed.
 
   Context `{i : heapG Σ} (L : namespace).
 
@@ -229,8 +219,7 @@ Section logrel.
     {|
       cofe_mor_car := λ τi, (∃ v, l ↦ v ★ (τi v))%I
     |}.
-  Next Obligation.
-  Proof. intros ???? H; apply exist_ne =>w; rewrite H; trivial. Qed.
+  Next Obligation. intros ???? H; apply exist_ne =>w; rewrite H; trivial. Qed.
 
   Program Definition interp_ref :
     (valC -n> iPropG lang Σ) -n> valC -n> iPropG lang Σ :=
@@ -241,10 +230,8 @@ Section logrel.
             λ w, (∃ l, w = LocV l ∧ inv (L .@ l) (interp_ref_pred l τi))%I
         |}
     |}.
+  Next Obligation. intros ???? H; rewrite H; trivial. Qed.
   Next Obligation.
-  Proof. intros ???? H; rewrite H; trivial. Qed.
-  Next Obligation.
-  Proof.
     intros ??? H ?; apply exist_ne=>w; apply and_ne; trivial; cbn.
     apply (contractive_ne _); apply exist_ne=>w'; rewrite H; trivial.
   Qed.
@@ -273,41 +260,23 @@ Section logrel.
   Solve Obligations
   with repeat intros ?; match goal with [H : _ ≡{_}≡ _|- _] => rewrite H end; trivial.
 
-  Class context_interp_Persistent (Δ : varC -n> valC -n> iPropG lang Σ) :=
-    contextinterppersistent : ∀ v : var, Val_to_IProp_Persistent (Δ v).
-
-  Global Instance Val_to_IProp_Persistent_Persistent
-         (f : valC -n> iPropG lang Σ)
-         {Hf : Val_to_IProp_Persistent f}
-         (v : val)
-    : PersistentP (f v).
-  Proof. apply Hf. Qed.
-
   Global Instance interp_Persistent
          τ (Δ : varC -n> valC -n> iPropG lang Σ)
-         {HΔ : context_interp_Persistent Δ}
-    : Val_to_IProp_Persistent (interp τ Δ).
+         {HΔ : ∀ x v, PersistentP (Δ x v)}
+    : ∀ v, PersistentP (interp τ Δ v).
   Proof.
     revert Δ HΔ.
     induction τ; cbn; intros Δ HΔ v; try apply _.
-    - rewrite /PersistentP /interp_rec fixpoint_unfold /interp_rec_pre; cbn.
-      apply always_intro'; trivial.
-    - apply Val_to_IProp_Persistent_Persistent; apply HΔ.
+    rewrite /PersistentP /interp_rec fixpoint_unfold /interp_rec_pre; cbn.
+    apply always_intro'; trivial.
   Qed.
 
-  Global Instance Persistent_context_interp_rel Δ Γ vs
-           {HΔ : context_interp_Persistent Δ}
-    : PersistentP ([∧] zip_with(λ τ v, interp τ Δ v) Γ vs)%I.
-  Proof. typeclasses eauto. Qed.
-
-  Global Program Instance extend_context_interp_Persistent f Δ
-           (Hf : Val_to_IProp_Persistent f)
-           {HΔ : context_interp_Persistent Δ}
-    : context_interp_Persistent (@extend_context_interp f Δ).
-  Next Obligation.
-    intros f Δ Hf HΔ v w; destruct v; cbn; trivial.
-    apply HΔ.
-  Qed.
+  Global Instance extend_context_interp_Persistent
+    (f : valC -n> iPropG lang Σ) (Δ : varC -n> valC -n> iPropG lang Σ)
+           (Hf : ∀ v, PersistentP (f v))
+           {HΔ : ∀ x v, PersistentP (Δ x v)}
+    : ∀ x v, PersistentP (@extend_context_interp f Δ x v).
+  Proof. intros x v. destruct x; cbn; trivial. Qed.
 
   Local Ltac properness :=
     repeat
@@ -380,10 +349,8 @@ Section logrel.
          λ Δ,
          {| cofe_mor_car := λ v, if lt_dec v m then Δ v else Δ (v - n) |}
     |}.
+  Next Obligation. intros ?????? Hxy; destruct Hxy; trivial. Qed.
   Next Obligation.
-  Proof. intros ?????? Hxy; destruct Hxy; trivial. Qed.
-  Next Obligation.
-  Proof.
     intros ????? Hfg ?; cbn. destruct lt_dec; rewrite Hfg; trivial.
   Qed.
 
@@ -474,12 +441,10 @@ Section logrel.
   Next Obligation.
   Proof. intros m τi Δ n x y Hxy; destruct Hxy; trivial. Qed.
   Next Obligation.
-  Proof.
     intros m τi n Δ Δ' HΔ x; cbn;
       destruct lt_dec; try destruct eq_nat_dec; auto.
   Qed.
   Next Obligation.
-  Proof.
     intros m n f g Hfg F Δ x; cbn;
       destruct lt_dec; try destruct eq_nat_dec; auto.
   Qed.
@@ -579,8 +544,8 @@ Section logrel.
   Lemma zip_with_context_interp_subst
         (Δ : varC -n> valC -n> iPropG lang Σ) (Γ : list type)
         (vs : list valC) (τi : valC -n> iPropG lang Σ) :
-    (([∧] zip_with (λ τ v, interp τ Δ v) Γ vs)%I)
-      ≡ ([∧] zip_with (λ τ v, interp τ (extend_context_interp τi Δ) v)
+    (([∧] zip_with (λ τ, interp τ Δ) Γ vs)%I)
+      ≡ ([∧] zip_with (λ τ, interp τ (extend_context_interp τi Δ))
                     (map (λ t : type, t.[ren (+1)]) Γ) vs)%I.
   Proof.
     revert Δ vs τi.
